\documentclass{standalone}
\usepackage{amsmath}
\begin{document}
$\begin{aligned}
&\alpha_{A}\cdot D_{0,\, 0.3,\, 1,\, 1}(C, \overline{T})+ \alpha_{F}\cdot D_{0,\, 0,\, 1,\, 1}(C_{0}, C)\\  
&= \alpha_{A}\cdot\sum_{i=1}^{n} d_{0,\, 0.3,\, 1,\, 1}(C, \overline{T}, \lbrace s_{i}, \neg s_{i}\rbrace) + \alpha_{F}\cdot\sum_{i=1}^{n} d_{0,\, 0,\, 1,\, 1}(C_{0}, C, \lbrace s_{i}, \neg s_{i}\rbrace)\\
&= \sum_{i=1}^{n} \alpha_{A}\cdot d_{0,\, 0.3,\, 1,\, 1}(C, \overline{T}, \lbrace s_{i}, \neg s_{i}\rbrace) + \alpha_{F}\cdot d_{0,\, 0,\, 1,\, 1}(C_{0}, C, \lbrace s_{i}, \neg s_{i}\rbrace)
\end{aligned}$
\end{document}